bdep working

proof/correctness1024/avx2/MLKEM_avx2_equivs.ec
@@ -36,6 +36,294 @@ import MLKEM_PolyAVX.
 import MLKEM_PolyvecAVX.
 import MLKEM_PolyAVXVec.
 import MLKEM_PolyVecAVXVec.
+
+require import Bindings.
+
+module DecompressBridge = {
+   proc __i_polyvec_decompress(r : W16.t Array1024.t, rp : W8.t Array1408.t, rrp : W8.t Array160.t) :  W16.t Array1024.t = {
+      var rp0 :  W8.t Array1568.t;
+      rp0 <- init_1568_8 (fun i => if 0 <= i < 1408 then rp.[i] else rrp.[i-1408]);
+      r <@ Jkem1024_avx2.M.__i_polyvec_decompress(r,rp0);
+      return r;
+  } 
+}.
+
+import KMatrix Vector.
+
+
+(********** BEGIN BDEP PROOF OF DECOMPRESS **************)
+
+op decompress11_circuit(c : W11.t) : W16.t = 
+  truncateu16 (srl_32 (((zeroextu11_32 c) * W32.of_int 3329) + W32.of_int 1024) (W32.of_int 11)).
+
+op pcond_true11(_: W11.t) = true.
+
+lemma polyvec_decompress_bridge_ll : islossless DecompressBridge.__i_polyvec_decompress.
+ proc; inline *;wp. 
+unroll for ^while.
+cfold ^inc<-.
+do 4!(unroll for ^while).
+auto.
+qed.
+
+from JazzEC require import WArray1568 WArray2048.
+require import Bindings BitEncoding.
+import BitChunking BS2Int.
+
+
+lemma polyvec_decompress_bridge_corr_h (_aw : W8.t Array1408.t):
+    hoare[ DecompressBridge.__i_polyvec_decompress :
+             rp = _aw ==> pos_bound1024_cxq res 0 1024 1 /\ lift_polyvec res = decompress_polyvec 11 (decode11_vec _aw)].
+proc; inline *.
+proc change 4: (sliceget16_16_256 jqx16 0); 1: by auto.
+proc change 5: (sliceget32_8_256 pvd_shufbidx_s 0); 1: by auto.
+proc change 6: (sliceget8_32_256 pvd_srlvdidx_s 0); 1: by auto.
+proc change 7: (sliceget4_64_256 pvd_srlvqidx_s 0); 1: by auto.
+proc change 8: (sliceget16_16_256 pvd_shift_s 0); 1: by auto.
+proc change ^while.^while.1 : (
+   if 0 <= (352*k + 22*i)*8 < 1568*8-256
+   then sliceget1568_8_256 rp1 ((352*k + 22*i)*8)
+   else get256_direct (WArray1568.init8 (fun (i_0 : int) => rp1.[i_0])) (352 * k + 22 * i)).
++ move => &hr.
+  case (0 <= (352 * k{hr} + 22 * i{hr}) * 8 < 1568 * 8 - 256); last by auto.
+  by move => *; rewrite /sliceget1568_8_256 ifT 1:/# /#.
+proc change ^while.^while.10 : (
+   if 0 <= (16 * k + i)*16 < 1024*16-256
+   then sliceset1024_16_256 r0 ((16 * k + i)*256) f
+   else Array1024.init   (fun (i0 : int) =>   
+      WArray2048.get16     
+         (WArray2048.set256 (WArray2048.init16 (fun (i_0 : int) => r0.[i_0])) (16 * k + i) f) i0)).
++ move => &hr.
+  case ( 0 <= (16 * k{hr} + i{hr})*16 < 1024*16-256); last by auto.
+  move => *; rewrite /sliceset1024_16_256 ifT 1:/#  /#.
+unroll for ^while.
+cfold ^inc<-.
+do 4!(unroll for ^while).
+cfold ^i<-.
+wp -4.
+bdep 11 16 [_aw] [rp] [r0] decompress11_circuit pcond_true11. 
+
+
+(* BDEP pre conseq *)
++ by move => &hr />; rewrite allP /pcond_true11 /=. 
+
+(* BDEP post conseq *)
+
+(* We start with some boilerplate *)
+move => &hr [#]/= <- rr; rewrite /= !flatten1.
+move => H1; have H2 := post_lane_commute_out_aligned (to_list rp{hr}) (to_list rr) W8.w2bits W8.bits2w W11.w2bits W11.bits2w W16.w2bits W16.bits2w  decompress11_circuit 8 11 16 _ _ _ _ _ _ _ _ _ _ _ _ H1;1..12:
+smt(Array1408.size_to_list Array1024.size_to_list W16.bits2wK BVA_Top_Bindings_W11_t.oflistP).
+
+have H3 : 
+   map decompress11_circuit (map W11.bits2w (chunk 11 (flatten (map W8.w2bits (to_list rp{hr}))))) =
+   map (W16.of_int \o asint) (to_list (decompress_polyvec 11 (decode11_vec rp{hr})).[0] ++ 
+                              to_list (decompress_polyvec 11 (decode11_vec rp{hr})).[1] ++ 
+                              to_list (decompress_polyvec 11 (decode11_vec rp{hr})).[2] ++ 
+                              to_list (decompress_polyvec 11 (decode11_vec rp{hr})).[3])%Vector.
++ rewrite /decode11_vec /decompress_polyvec !map_cat !setvE !offunvE 1..4:/# /= !offunvK /vclamp /kvec /= /subarray256 /=.
+  apply (eq_from_nth witness).
+  + rewrite !size_map !size_cat !size_map !size_iota /max /=.
+     rewrite (EclibExtra.size_flatten' 8);1:smt(mapP W8.size_w2bits). 
+     by rewrite size_map size_to_list /=.
+  move => i.
+  rewrite !size_map size_iota.
+  rewrite (EclibExtra.size_flatten' 8);1:smt(mapP W8.size_w2bits). 
+   rewrite size_map size_to_list /max  /= => ib.
+  rewrite !nth_cat !size_map !size_cat !size_map !size_iota /max /=. 
+  case (i <256).
+  + move => ?;rewrite ifT 1:/# ifT 1:/#.
+    rewrite (nth_map witness).
+    + rewrite size_map size_chunk 1:/# (EclibExtra.size_flatten' 8);1:smt(mapP W8.size_w2bits). 
+      rewrite size_map size_to_list /= /#.
+    rewrite (nth_map []).
+    + rewrite  size_chunk 1:/# (EclibExtra.size_flatten' 8);1:smt(mapP W8.size_w2bits). 
+      rewrite size_map size_to_list /= /#.
+    rewrite (nth_map witness _ ((W16.of_int \o asint))) /=.
+    + rewrite size_to_list /= /#.
+   rewrite /(\o) /= mapiE 1:/# /= initiE 1:/# /=.  
+  rewrite /(\o) /decompress11_circuit -decompress_alt_decompress /decompress_alt //=.
+  rewrite get_of_list 1:/# /= qE /=.
+  have Hs := size_nth_chunk [] (flatten (map W8.w2bits (to_list rp{hr}))) i 11 _ _ => //.
+  + rewrite (EclibExtra.size_flatten' 8);1:smt(mapP W8.size_w2bits). 
+    by rewrite size_map size_to_list /#.
+  rewrite to_uint_eq to_uint_truncateu16 /= /srl_32 /= of_uintK /=;congr;congr.
+  have ? : 2^11 = 2048 by auto.
+  rewrite to_uint_shr //= /zeroextu11_32 to_uintD_small /=;1: by rewrite of_uintK /=; smt(modz_small W11.to_uint_cmp). 
+  rewrite of_uintK /= modz_small;1:by smt( W11.to_uint_cmp). 
+  rewrite /to_uint bits2wK 1:/# incoeffK qE /= /decode (nth_map [] _ bs2int) /=.
+  + rewrite size_chunk 1:/# size_BytesToBits size_to_list /= /#.
+  by smt(BS2Int.bs2int_ge0 BS2Int.bs2int_le2Xs modz_small W11.to_uint_cmp). 
+
+  case (i <512).
+  + move => ??;rewrite ifT 1:/#.
+    rewrite (nth_map witness).
+    + rewrite size_map size_chunk 1:/# (EclibExtra.size_flatten' 8);1:smt(mapP W8.size_w2bits). 
+      rewrite size_map size_to_list /= /#.
+    rewrite (nth_map []).
+    + rewrite  size_chunk 1:/# (EclibExtra.size_flatten' 8);1:smt(mapP W8.size_w2bits). 
+      rewrite size_map size_to_list /= /#.
+    rewrite (nth_map witness _ ((W16.of_int \o asint))) /=.
+    + rewrite size_to_list /= /#.
+   rewrite /(\o) /= mapiE 1:/# /= initiE 1:/# /=.  
+  rewrite /(\o) /decompress11_circuit -decompress_alt_decompress /decompress_alt //=.
+  rewrite get_of_list 1:/# /= qE /=.
+  have Hs := size_nth_chunk [] (flatten (map W8.w2bits (to_list rp{hr}))) i 11 _ _ => //.
+  + rewrite (EclibExtra.size_flatten' 8);1:smt(mapP W8.size_w2bits). 
+    by rewrite size_map size_to_list /#.
+  rewrite to_uint_eq to_uint_truncateu16 /= /srl_32 /= of_uintK /=;congr;congr.
+  have ? : 2^11 = 2048 by auto.
+  rewrite to_uint_shr //= /zeroextu11_32 to_uintD_small /=;1: by rewrite of_uintK /=; smt(modz_small W11.to_uint_cmp). 
+  rewrite of_uintK /= modz_small;1:by smt( W11.to_uint_cmp). 
+  rewrite /to_uint bits2wK 1:/# incoeffK qE /= /decode (nth_map [] _ bs2int) /=.
+  + rewrite size_chunk 1:/# size_BytesToBits size_to_list /= /#.
+  by smt(BS2Int.bs2int_ge0 BS2Int.bs2int_le2Xs modz_small W11.to_uint_cmp). 
+
+  case (i <768).
+  + move => ???.
+    rewrite (nth_map witness).
+    + rewrite size_map size_chunk 1:/# (EclibExtra.size_flatten' 8);1:smt(mapP W8.size_w2bits). 
+      rewrite size_map size_to_list /= /#.
+    rewrite (nth_map []).
+    + rewrite  size_chunk 1:/# (EclibExtra.size_flatten' 8);1:smt(mapP W8.size_w2bits). 
+      rewrite size_map size_to_list /= /#.
+    rewrite (nth_map witness _ ((W16.of_int \o asint))) /=.
+    + rewrite size_to_list /= /#.
+   rewrite /(\o) /= mapiE 1:/# /= initiE 1:/# /=.  
+  rewrite /(\o) /decompress11_circuit -decompress_alt_decompress /decompress_alt //=.
+  rewrite get_of_list 1:/# /= qE /=.
+  have Hs := size_nth_chunk [] (flatten (map W8.w2bits (to_list rp{hr}))) i 11 _ _ => //.
+  + rewrite (EclibExtra.size_flatten' 8);1:smt(mapP W8.size_w2bits). 
+    by rewrite size_map size_to_list /#.
+  rewrite to_uint_eq to_uint_truncateu16 /= /srl_32 /= of_uintK /=;congr;congr.
+  have ? : 2^11 = 2048 by auto.
+  rewrite to_uint_shr //= /zeroextu11_32 to_uintD_small /=;1: by rewrite of_uintK /=; smt(modz_small W11.to_uint_cmp). 
+  rewrite of_uintK /= modz_small;1:by smt( W11.to_uint_cmp). 
+  rewrite /to_uint bits2wK 1:/# incoeffK qE /= /decode (nth_map [] _ bs2int) /=.
+  + rewrite size_chunk 1:/# size_BytesToBits size_to_list /= /#.
+  by smt(BS2Int.bs2int_ge0 BS2Int.bs2int_le2Xs modz_small W11.to_uint_cmp). 
+
+  + move => ???.
+    rewrite (nth_map witness).
+    + rewrite size_map size_chunk 1:/# (EclibExtra.size_flatten' 8);1:smt(mapP W8.size_w2bits). 
+      rewrite size_map size_to_list /= /#.
+    rewrite (nth_map []).
+    + rewrite  size_chunk 1:/# (EclibExtra.size_flatten' 8);1:smt(mapP W8.size_w2bits). 
+      rewrite size_map size_to_list /= /#.
+    rewrite (nth_map witness _ ((W16.of_int \o asint))) /=.
+    + rewrite size_to_list /= /#.
+   rewrite /(\o) /= mapiE 1:/# /= initiE 1:/# /=.  
+  rewrite /(\o) /decompress11_circuit -decompress_alt_decompress /decompress_alt //=.
+  rewrite get_of_list 1:/# /= qE /=.
+  have Hs := size_nth_chunk [] (flatten (map W8.w2bits (to_list rp{hr}))) i 11 _ _ => //.
+  + rewrite (EclibExtra.size_flatten' 8);1:smt(mapP W8.size_w2bits). 
+    by rewrite size_map size_to_list /#.
+  rewrite to_uint_eq to_uint_truncateu16 /= /srl_32 /= of_uintK /=;congr;congr.
+  have ? : 2^11 = 2048 by auto.
+  rewrite to_uint_shr //= /zeroextu11_32 to_uintD_small /=;1: by rewrite of_uintK /=; smt(modz_small W11.to_uint_cmp). 
+  rewrite of_uintK /= modz_small;1:by smt( W11.to_uint_cmp). 
+  rewrite /to_uint bits2wK 1:/# incoeffK qE /= /decode (nth_map [] _ bs2int) /=.
+  + rewrite size_chunk 1:/# size_BytesToBits size_to_list /= /#.
+  by smt(BS2Int.bs2int_ge0 BS2Int.bs2int_le2Xs modz_small W11.to_uint_cmp). 
+
+
+split; last first.
++ rewrite eq_vectorP => i @/kvec ib.
+  rewrite /lift_polyvec /decompress_polyvec !setvE !offunvE 1..2:/# /= !offunvK /vclamp /kvec /= ib /=. 
+  case (3 = i) => Hi.
+  + rewrite tP => k kb. 
+    rewrite -Hi !mapiE 1,2:/# !initiE 1,2:/# /= /= -get_to_list H2 H3.
+  rewrite (nth_map witness);1: by smt(Array256.size_to_list size_cat).
+  rewrite (nth_cat witness).
+  + rewrite !size_cat !size_to_list /= ifF 1:/# /decompress_polyvec.
+    rewrite !setvE !offunvE 1:/# /=.
+    rewrite initiE 1:/# /= mapiE 1:/# initiE 1:/# /=.
+    rewrite get_of_list 1:/# /=.
+  pose c := (decompress 11 (nth 0 (decode 11 (to_list rp{hr})) (768 + k))).
+  rewrite of_sintK /= /smod /= ifF;1:smt(@Zq).
+  rewrite modz_small; smt(@Zq).  
+
+  case (2 = i) => Hi2.
+  + rewrite tP => k kb. 
+    rewrite -Hi2 !mapiE 1,2:/# !initiE 1,2:/# /= /= -get_to_list H2 H3.
+  rewrite (nth_map witness);1: by smt(Array256.size_to_list size_cat).
+  rewrite (nth_cat witness).
+  + rewrite !size_cat !size_to_list /= ifT 1:/# /decompress_polyvec.
+    rewrite !setvE !offunvE 1..3:/# /=  !offunvK /vclamp /= !ifT 1..6:/#.
+  rewrite (nth_cat witness).
+  + rewrite !size_cat !size_to_list /= ifF 1:/# /decompress_polyvec.
+    rewrite  mapiE 1:/# initiE 1:/# /= initiE 1:/# /=.
+    rewrite of_sintK /= /smod /= ifF;1:smt(@Zq).
+  pose c := decompress 11 (nth 0 (decode 11 (to_list rp{hr})) (512 + k)).
+  rewrite modz_small; smt(@Zq).  
+
+  case (1 = i) => Hi1.
+  + rewrite tP => k kb. 
+    rewrite -Hi1 !mapiE 1,2:/# !initiE 1,2:/# /= /= -get_to_list H2 H3.
+  rewrite (nth_map witness);1: by smt(Array256.size_to_list size_cat).
+  rewrite (nth_cat witness).
+  + rewrite !size_cat !size_to_list /= ifT 1:/# /decompress_polyvec.
+    rewrite !setvE !offunvE 1..3:/# /= !offunvK /vclamp /= !ifT 1..6:/#.
+  rewrite (nth_cat witness).
+  + rewrite !size_cat !size_to_list /= ifT 1:/# /decompress_polyvec.
+  rewrite (nth_cat witness).
+  + rewrite !size_to_list /= ifF 1:/# /decompress_polyvec.
+    rewrite  mapiE 1:/# initiE 1:/# /= initiE 1:/# /=.
+    rewrite of_sintK /= /smod /= ifF;1:smt(@Zq).
+    pose c := (decompress 11 (nth 0 (decode 11 (to_list rp{hr})) (256 + k))).
+  rewrite modz_small; smt(@Zq).  
+
+  have Hi3 :(0 = i) by smt().
+  + rewrite tP => k kb.
+    rewrite -Hi3 /= !mapiE 1,2:/# /= initiE 1:/# /= -( Array1024.get_to_list rr) H2 H3.
+  rewrite (nth_map witness);1: by smt(Array256.size_to_list size_cat).
+  rewrite (nth_cat witness).
+  + rewrite !size_cat !size_to_list /= ifT 1:/# /decompress_polyvec.
+    rewrite !setvE !offunvE 1..3:/# /= !offunvK /vclamp /= !ifT 1..6:/#.
+  rewrite (nth_cat witness).
+  + rewrite !size_cat !size_to_list /= ifT 1:/# /decompress_polyvec.
+  rewrite (nth_cat witness).
+  + rewrite !size_to_list /= ifT 1:/# /decompress_polyvec.
+    rewrite  mapiE 1:/# initiE 1:/# /= initiE 1:/# /=.
+    rewrite of_sintK /= /smod /= ifF;1:smt(@Zq).
+    pose c := (decompress 11 (nth 0 (decode 11 (to_list rp{hr})) (k))).
+  rewrite modz_small; smt(@Zq).  
+
+
+rewrite /pos_bound1024_cxq qE /= => k kb. 
+rewrite -get_to_list  H2 H3 /decompress_poly.
+rewrite (nth_map witness);1: by smt(size_cat Array256.size_to_list).
+rewrite (nth_cat witness) !size_cat !size_to_list /=. 
+rewrite (nth_cat witness) !size_cat !size_to_list /=. 
+rewrite (nth_cat witness)  !size_to_list /=. 
+rewrite /decompress_polyvec !setvE /= !offunvE 1..4:/# /= !offunvK /= /vclamp /kvec/=.
+case (k < 256).
++ move => *; rewrite ifT 1:/# .
+  rewrite mapiE 1:/# initiE 1:/# /=.
+  rewrite of_sintK /= /smod /= ifF;1:smt(@Zq).
+  rewrite modz_small; smt(@Zq).  
+case (k < 512).
++ move => *.
+  rewrite mapiE 1:/# initiE 1:/# /=.
+  rewrite of_sintK /= /smod /= ifF;1:smt(@Zq).
+  rewrite modz_small; smt(@Zq).  
+case (k < 768).
++ move => *.
+  rewrite mapiE 1:/# initiE 1:/# /=.
+  rewrite of_sintK /= /smod /= ifF;1:smt(@Zq).
+  rewrite modz_small; smt(@Zq).  
++ move => *.
+  rewrite mapiE 1:/# initiE 1:/# /=.
+  rewrite of_sintK /= /smod /= ifF;1:smt(@Zq).
+  rewrite modz_small; smt(@Zq).  
+
+qed.
+
+
+lemma polyvec_decompress_bridge_corr (_aw : W8.t Array1408.t):
+    phoare[ DecompressBridge.__i_polyvec_decompress :
+             rp = _aw ==> pos_bound1024_cxq res 0 1024 1 /\ lift_polyvec res = decompress_polyvec 11 (decode11_vec _aw)] = 1%r
+ by conseq polyvec_decompress_bridge_ll (polyvec_decompress_bridge_corr_h _aw).
+
 lemma polyvec_decompress_equiv  :
     equiv [Jkem1024_avx2.M.__i_polyvec_decompress ~  Jkem1024.M.__i_polyvec_decompress  :
              Array1408.init(fun i => arg{1}.`2.[i]) =arg{2}.`2
@@ -43,7 +331,44 @@ lemma polyvec_decompress_equiv  :
              lift_array1024 res{1} = lift_array1024 res{2} /\
              pos_bound1024_cxq res{1} 0 1024 1 /\
              pos_bound1024_cxq res{2} 0 1024 1 ].
-admitted.
+proc*. 
+transitivity {1} {r0<@ DecompressBridge.__i_polyvec_decompress(r,Array1408.init(fun i => rp.[i]), Array160.init(fun i => rp.[i+1408]));}
+    (={rp,r} ==> ={r0})
+    (Array1408.init(fun i => rp{1}.[i]) = ap{2}
+      ==> lift_array1024 r0{1} = lift_array1024 r{2} /\
+             pos_bound1024_cxq r0{1} 0 1024 1 /\
+             pos_bound1024_cxq r{2} 0 1024 1); 1,2:smt().
+inline {2} 1;sim;auto => /> &1. 
++ rewrite /init_1568_8 tP => i*.
+  rewrite initiE 1:/# /=.
+  case (0 <= i < 1408) => *; rewrite initiE 1:/# /= /#.
+  
+ecall {2} (polyvec_decompress_corr ap{2}) => /=.
+ecall {1} (polyvec_decompress_bridge_corr (Array1408.init (fun (i : int) => rp{1}.[i]))).
++ auto => /> &1 r1 ? <- rr ?; rewrite /lift_array1024 /lift_polyvec /lift_array256 /subarray256 !eq_vectorP /kvec tP =>H i ib.
+  rewrite !mapiE 1,2:/# /=.
+  case (0<= i < 256) => Hi0.
+  + have  := (H 0 _);1:by auto.
+    rewrite !offunvE /= /kvec //= tP => Hi.
+    by have := (Hi i Hi0); rewrite !mapiE 1,2:/# /= initiE 1:/# /= initiE 1:/# /= /#.
+  case (256<= i < 512) => Hi1.
+  + have  := (H 1 _);1:by auto.
+    rewrite !offunvE /= /kvec //= tP => Hi.
+    have := (Hi (i - 256) _); 1:smt(). 
+    by rewrite !mapiE 1,2:/# /= initiE 1:/# /= initiE 1:/# /= /#.
+  case (512<= i < 768) => Hi2.
+  + have  := (H 2 _);1:by auto.
+    rewrite !offunvE /= /kvec //= tP => Hi.
+    have := (Hi (i - 512) _); 1:smt(). 
+    by rewrite !mapiE 1,2:/# /= initiE 1:/# /= initiE 1:/# /= /#.
+  have Hi3 :  (768<= i < 1024)  by smt().
+    have  := (H 3 _);1:by auto.
+    rewrite !offunvE /= /kvec //= tP => Hi.
+    have := (Hi (i - 768) _); 1:smt(). 
+    by rewrite !mapiE 1,2:/# /= initiE 1:/# /= initiE 1:/# /= /#.
+qed.
+
+(***********************)
 
 equiv compressequivvec  : 
  Jkem1024_avx2.M.__i_polyvec_compress ~  Jkem1024.M.__i_polyvec_compress :
